@prefix adms: <http://www.w3.org/ns/adms#> .
@prefix dcat: <http://www.w3.org/ns/dcat#> .
@prefix dct: <http://purl.org/dc/terms/> .
@prefix dqv: <http://www.w3.org/ns/dqv#> .
@prefix foaf: <http://xmlns.com/foaf/0.1/> .
@prefix geodcat: <http://data.europa.eu/930/> .
@prefix gsp:  <http://www.opengis.net/ont/geosparql#>.
@prefix profile: <https://ex.org/profile/#> .
@prefix : <https://ex.org/#> .
@prefix gkc: <https://geokur-dmp.geo.tu-dresden.de/category-register#> .
@prefix gkq: <https://geokur-dmp.geo.tu-dresden.de/quality-register#> .
@prefix gsp: <http://www.opengis.net/ont/geosparql#> .
@prefix locn: <http://www.w3.org/ns/locn#> .
@prefix oa: <https://www.w3.org/TR/annotation-vocab#> .
@prefix owl: <http://www.w3.org/2002/07/owl#> .
@prefix prov: <http://www.w3.org/ns/prov#> .
@prefix rdf: <http://www.w3.org/1999/02/22-rdf-syntax-ns#> .
@prefix rdfs: <http://www.w3.org/2000/01/rdf-schema#> .
@prefix schema: <http://schema.org/> .
@prefix sdmx: <http://purl.org/linked-data/sdmx/2009/attribute#> .
@prefix skos: <http://www.w3.org/2004/02/skos/core#> .
@prefix spdx: <http://spdx.org/rdf/terms#> .
@prefix time: <http://www.w3.org/2006/time> .
@prefix vcard: <http://www.w3.org/2006/vcard/ns#> .
@prefix xml: <http://www.w3.org/XML/1998/namespace> .
@prefix xsd: <http://www.w3.org/2001/XMLSchema#> .
@prefix fao: <https://www.fao.org/home/en/#> .
@prefix gez2010_geoms: <https://github.com/rue-a/dqv_inhomogeneity/blob/master/gaez_2010_geometries/> .

:periodFrom2000to2012 a dct:PeriodOfTime , time:ProperInterval ;
    time:hasBeginning [ 
        a time:Instant ;
        time:inXSDgYear "2000"^^xsd:gYear ;
    ];
    time:hasEnd [ 
        a time:Instant ;
        time:inXSDgYear "2012"^^xsd:gYear ;
    ] .

:forest a skos:Concept ;
    skos:prefLabel "Forest"@en ;
    skos:definition "\" [...] forest cover is defined as 25% or greater canopy closure at the Landsat pixel scale (30-m × 30-m spatial resolution) for trees >5 m in height.\" [https://www.pnas.org/doi/10.1073/pnas.0912668107]"@en .

:forestChange a skos:Concept ;
    skos:prefLabel "Forest Change"@en ;
    skos:definition "Forest gain minus forest loss"@en ;
    skos:related :forest  .

:forestGain a skos:Concept ;
    skos:prefLabel "Forest Gain"@en ;
    skos:definition "\"Forest gain was defined as the inverse of loss, or the establishment of tree canopy from a nonforest state.\" [https://www.science.org/doi/epdf/10.1126/science.1244693]"@en ;
    skos:related :forest ;
    skos:narrower :forestChange .

:forestLoss a skos:Concept ;
    skos:prefLabel "Forest Loss"@en ;
    skos:definition "\"Forest loss was defined as a stand-replacement disturbance or the complete removal of tree cover canopy at the Landsat pixel scale.\" [https://www.science.org/doi/epdf/10.1126/science.1244693]"@en ;
    skos:related :forest  ;
    skos:narrower :forestChange .

:forestNoGain a skos:Concept ;
    skos:prefLabel "Forest No Gain"@en ;
    skos:definition "Areas where no Forest Gain was identified (spatial complement of forest gain)"@en ;
    skos:related :forest .

:forestNoLoss a skos:Concept ;
    skos:prefLabel "Forest No Loss"@en ;
    skos:definition "Areas where no Forest Loss was identified (spatial complement of forest loss)"@en ;
    skos:related :forest .


:globalForestChange a dcat:Dataset,
        prov:Entity;
    dct:description "Results from time-series analysis of Landsat images characterizing forest extent and change."@en ;
    dct:issued "2022-01-20T11:20:48.837328"^^xsd:dateTime ;
    dct:modified "2022-03-21T12:38:14.007818"^^xsd:dateTime ;
    dct:temporal [ a dct:PeriodOfTime ,  time:ProperInterval ;
        time:hasBeginning [ 
            a time:Instant ;
            time:inXSDgYear "2000"^^xsd:gYear ;
        ];
        time:hasEnd [ 
            a time:Instant ;
            time:inXSDgYear "2020"^^xsd:gYear ;
        ] 
    ];
    dct:spatial [ a dct:Location, gsp:Feature;
    gsp:hasDefaultGeometry [
            gsp:asWKT "POLYGON((-180 -90,-180 90,180 90,180 -90,-180 -90))"^^gsp:wktLiteral 
        ] 
    ];
    dct:title "Global Forest Change"@en ;
    dcat:contactPoint :globalForestChangeAuthor ;
    dcat:keyword "deforestation"@en,
        "forest"@en,
        "forest cover change"@en,
        "global"@en,
        "tree"@en ;
    dcat:landingPage <https://glad.earthengine.app/view/global-forest-change#dl=1%3Bold=off%3Bbl=off%3Blon=20%3Blat=10%3Bzoom=3%3B> ;
    dcat:spatialResolutionInMeters 30.0 ;
    dcat:temporalResolution "annual"^^xsd:duration ;
    dqv:hasQualityMeasurement
        

        # TROPICAL FOREST GAIN error matrix (user's and producer's accuracy values) from 2000 to 2012 
        [ a dqv:QualityMeasurement ;
            dct:temporal :periodFrom2000to2012 ;
            dct:spatial fao:globalEcologicalZones2010Tropical ;
            dqv:isMeasurementOf gkq:UsersAccuracy ;
            dqv:value "81.9"^^xsd:double ;
            profile:thematic :forestGain ],
        [ a dqv:QualityMeasurement ;
            dct:temporal :periodFrom2000to2012 ;
            dct:spatial fao:globalEcologicalZones2010Tropical ;
            dqv:isMeasurementOf gkq:ProducersAccuracy ;
            dqv:value "48.0"^^xsd:double ;
            profile:thematic :forestGain ],
        [ a dqv:QualityMeasurement ;
            dct:temporal :periodFrom2000to2012 ;
            dct:spatial fao:globalEcologicalZones2010Tropical ;
            dqv:isMeasurementOf gkq:UsersAccuracy ;
            dqv:value "99.8"^^xsd:double ;
            profile:thematic :forestNoGain ] ,
        [ a dqv:QualityMeasurement ;
            dct:temporal :periodFrom2000to2012 ;
            dct:spatial fao:globalEcologicalZones2010Tropical ;
            dqv:isMeasurementOf gkq:ProducersAccuracy ;
            dqv:value "99.9"^^xsd:double ;
            profile:thematic :forestNoGain ],        
        
        # TROPICAL FOREST LOSS error matrix (user's and producer's accuracy values) from 2000 to 2012 
        [ a dqv:QualityMeasurement ;
            dct:temporal :periodFrom2000to2012 ;
            dct:spatial fao:globalEcologicalZones2010Tropical ;
            dqv:isMeasurementOf gkq:UsersAccuracy ;
            dqv:value "87.0"^^xsd:double ;
            profile:thematic :forestLoss ],
        [ a dqv:QualityMeasurement ;
            dct:temporal :periodFrom2000to2012 ;
            dct:spatial fao:globalEcologicalZones2010Tropical ;
            dqv:isMeasurementOf gkq:ProducersAccuracy ;
            dqv:value "83.1"^^xsd:double ;
            profile:thematic :forestLoss ],
        [ a dqv:QualityMeasurement ;
            dct:temporal :periodFrom2000to2012 ;
            dct:spatial fao:globalEcologicalZones2010Tropical ;
            dqv:isMeasurementOf gkq:UsersAccuracy ;
            dqv:value "99.7"^^xsd:double ;
            profile:thematic :forestNoLoss ],
        [ a dqv:QualityMeasurement ;
            dct:temporal :periodFrom2000to2012 ;
            dct:spatial fao:globalEcologicalZones2010Tropical ;
            dqv:isMeasurementOf gkq:ProducersAccuracy ;
            dqv:value "99.8"^^xsd:double ;
            profile:thematic :forestNoLoss ],


    # SUBTROPICAL FOREST GAIN error matrix (user's and producer's accuracy values) from 2000 to 2012 
        [ a dqv:QualityMeasurement ;
            dct:temporal :periodFrom2000to2012 ;
            dct:spatial fao:globalEcologicalZones2010Subtropical ;
            dqv:isMeasurementOf gkq:UsersAccuracy ;
            dqv:value "85.5"^^xsd:double ;
            profile:thematic :forestGain ],
        [ a dqv:QualityMeasurement ;
            dct:temporal :periodFrom2000to2012 ;
            dct:spatial fao:globalEcologicalZones2010Subtropical ;
            dqv:isMeasurementOf gkq:ProducersAccuracy ;
            dqv:value "82.4"^^xsd:double ;
            profile:thematic :forestGain ],
        [ a dqv:QualityMeasurement ;
            dct:temporal :periodFrom2000to2012 ;
            dct:spatial fao:globalEcologicalZones2010Subtropical ;
            dqv:isMeasurementOf gkq:UsersAccuracy ;
            dqv:value "99.8"^^xsd:double ;
            profile:thematic :forestNoGain ] ,
        [ a dqv:QualityMeasurement ;
            dct:temporal :periodFrom2000to2012 ;
            dct:spatial fao:globalEcologicalZones2010Subtropical ;
            dqv:isMeasurementOf gkq:ProducersAccuracy ;
            dqv:value "99.9"^^xsd:double ;
            profile:thematic :forestNoGain ],        
        
        # SUBTROPICAL FOREST LOSS error matrix (user's and producer's accuracy values) from 2000 to 2012 
        [ a dqv:QualityMeasurement ;
            dct:temporal :periodFrom2000to2012 ;
            dct:spatial fao:globalEcologicalZones2010Subtropical ;
            dqv:isMeasurementOf gkq:UsersAccuracy ;
            dqv:value "79.3"^^xsd:double ;
            profile:thematic :forestLoss ],
        [ a dqv:QualityMeasurement ;
            dct:temporal :periodFrom2000to2012 ;
            dct:spatial fao:globalEcologicalZones2010Subtropical ;
            dqv:isMeasurementOf gkq:ProducersAccuracy ;
            dqv:value "79.4"^^xsd:double ;
            profile:thematic :forestLoss ],
        [ a dqv:QualityMeasurement ;
            dct:temporal :periodFrom2000to2012 ;
            dct:spatial fao:globalEcologicalZones2010Subtropical ;
            dqv:isMeasurementOf gkq:UsersAccuracy ;
            dqv:value "99.8"^^xsd:double ;
            profile:thematic :forestNoLoss ],
        [ a dqv:QualityMeasurement ;
            dct:temporal :periodFrom2000to2012 ;
            dct:spatial fao:globalEcologicalZones2010Subtropical ;
            dqv:isMeasurementOf gkq:ProducersAccuracy ;
            dqv:value "99.8"^^xsd:double ;
            profile:thematic :forestNoLoss ],


    # TEMPERATE FOREST GAIN error matrix (user's and producer's accuracy values) from 2000 to 2012 
        [ a dqv:QualityMeasurement ;
            dct:temporal :periodFrom2000to2012 ;
            dct:spatial fao:globalEcologicalZones2010Temperate ;
            dqv:isMeasurementOf gkq:UsersAccuracy ;
            dqv:value "62.0"^^xsd:double ;
            profile:thematic :forestGain ],
        [ a dqv:QualityMeasurement ;
            dct:temporal :periodFrom2000to2012 ;
            dct:spatial fao:globalEcologicalZones2010Temperate ;
            dqv:isMeasurementOf gkq:ProducersAccuracy ;
            dqv:value "76.5"^^xsd:double ;
            profile:thematic :forestGain ],
        [ a dqv:QualityMeasurement ;
            dct:temporal :periodFrom2000to2012 ;
            dct:spatial fao:globalEcologicalZones2010Temperate ;
            dqv:isMeasurementOf gkq:UsersAccuracy ;
            dqv:value "99.9"^^xsd:double ;
            profile:thematic :forestNoGain ] ,
        [ a dqv:QualityMeasurement ;
            dct:temporal :periodFrom2000to2012 ;
            dct:spatial fao:globalEcologicalZones2010Temperate ;
            dqv:isMeasurementOf gkq:ProducersAccuracy ;
            dqv:value "99.8"^^xsd:double ;
            profile:thematic :forestNoGain ],        
        
        # TEMPERATE FOREST LOSS error matrix (user's and producer's accuracy values) from 2000 to 2012 
        [ a dqv:QualityMeasurement ;
            dct:temporal :periodFrom2000to2012 ;
            dct:spatial fao:globalEcologicalZones2010Temperate ;
            dqv:isMeasurementOf gkq:UsersAccuracy ;
            dqv:value "88.2"^^xsd:double ;
            profile:thematic :forestLoss ],
        [ a dqv:QualityMeasurement ;
            dct:temporal :periodFrom2000to2012 ;
            dct:spatial fao:globalEcologicalZones2010Temperate ;
            dqv:isMeasurementOf gkq:ProducersAccuracy ;
            dqv:value "93.9"^^xsd:double ;
            profile:thematic :forestLoss ],
        [ a dqv:QualityMeasurement ;
            dct:temporal :periodFrom2000to2012 ;
            dct:spatial fao:globalEcologicalZones2010Temperate ;
            dqv:isMeasurementOf gkq:UsersAccuracy ;
            dqv:value "99.9"^^xsd:double ;
            profile:thematic :forestNoLoss ],
        [ a dqv:QualityMeasurement ;
            dct:temporal :periodFrom2000to2012 ;
            dct:spatial fao:globalEcologicalZones2010Temperate ;
            dqv:isMeasurementOf gkq:ProducersAccuracy ;
            dqv:value "99.9"^^xsd:double ;
            profile:thematic :forestNoLoss ],

        # BOREAL FOREST GAIN error matrix (user's and producer's accuracy values) from 2000 to 2012 
        [ a dqv:QualityMeasurement ;
            dct:temporal :periodFrom2000to2012 ;
            dct:spatial fao:globalEcologicalZones2010Boreal ;
            dqv:isMeasurementOf gkq:UsersAccuracy ;
            dqv:value "76.7"^^xsd:double ;
            profile:thematic :forestGain ],
        [ a dqv:QualityMeasurement ;
            dct:temporal :periodFrom2000to2012 ;
            dct:spatial fao:globalEcologicalZones2010Boreal ;
            dqv:isMeasurementOf gkq:ProducersAccuracy ;
            dqv:value "98.4"^^xsd:double ;
            profile:thematic :forestGain ],
        [ a dqv:QualityMeasurement ;
            dct:temporal :periodFrom2000to2012 ;
            dct:spatial fao:globalEcologicalZones2010Boreal ;
            dqv:isMeasurementOf gkq:UsersAccuracy ;
            dqv:value "99.9"^^xsd:double ;
            profile:thematic :forestNoGain ] ,
        [ a dqv:QualityMeasurement ;
            dct:temporal :periodFrom2000to2012 ;
            dct:spatial fao:globalEcologicalZones2010Boreal ;
            dqv:isMeasurementOf gkq:ProducersAccuracy ;
            dqv:value "99.7"^^xsd:double ;
            profile:thematic :forestNoGain ],        
        
        # BOREAL FOREST LOSS error matrix (user's and producer's accuracy values) from 2000 to 2012 
        [ a dqv:QualityMeasurement ;
            dct:temporal :periodFrom2000to2012 ;
            dct:spatial fao:globalEcologicalZones2010Boreal ;
            dqv:isMeasurementOf gkq:UsersAccuracy ;
            dqv:value "88.0"^^xsd:double ;
            profile:thematic :forestLoss ],
        [ a dqv:QualityMeasurement ;
            dct:temporal :periodFrom2000to2012 ;
            dct:spatial fao:globalEcologicalZones2010Boreal ;
            dqv:isMeasurementOf gkq:ProducersAccuracy ;
            dqv:value "93.9"^^xsd:double ;
            profile:thematic :forestLoss ],
        [ a dqv:QualityMeasurement ;
            dct:temporal :periodFrom2000to2012 ;
            dct:spatial fao:globalEcologicalZones2010Boreal ;
            dqv:isMeasurementOf gkq:UsersAccuracy ;
            dqv:value "99.8"^^xsd:double ;
            profile:thematic :forestNoLoss ],
        [ a dqv:QualityMeasurement ;
            dct:temporal :periodFrom2000to2012 ;
            dct:spatial fao:globalEcologicalZones2010Boreal ;
            dqv:isMeasurementOf gkq:ProducersAccuracy ;
            dqv:value "99.5"^^xsd:double ;
            profile:thematic :forestNoLoss ];

            

    prov:wasAttributedTo :globalForestChangeAuthor ;
    foaf:page <https://www.science.org/doi/10.1126/science.1244693> .


:globalForestChangeAuthor a prov:Agent ;
    vcard:fn "Hansen, M. C., P. V Potapov, R. Moore, M. Hancher, S. A. Turubanova, A. Tyukavina, D. Thau, S. V Stehman, S. J. Goetz, T. R. Loveland, A. Kommareddy, A. Egorov, L. Chini, C. O. Justice, and J. R. G. Townshend; University of Maryland, Department of geographical Science"@en .

fao:globalEcologicalZones a skos:Concept ;
    skos:definition """
Conventionally the Food and Agriculture Organization of the United Nations (FAO) reports forest statistics according to political divisions: Nations, Regions and Continents. Expert consultations to the FRA held in Kotka, Finland, provided a mandate for FAO to incorporate indicators of biodiversity into the Assessment (FAO, 2001). In response FAO developed the Global Ecological Zones (GEZ) classification and maps, which were used to present forest statistics including information on forest cover change. An Ecological Zone (EZ) is defined as:
 “A zone or area with broad yet relatively homogeneous natural vegetation formations, similar (not necessarily identical) in physiognomy. Boundaries of the EZs approximately coincide with the map of Köppen-Trewartha climatic types, which was based on temperature and rainfall. An exception to this definition are “Mountain systems”, classified as one separate EZ in each Domain and characterized by a high variation in both vegetation formations and climatic conditions caused by large altitude and topographic variation” [Simons, H. (2001) FRA 2000. Global Ecological Zoning for the Global Forest Resources Assessment 2000. FRA Working Paper 56. FAO, Rome.] [https://www.fao.org/3/ap861e/ap861e.pdf].
""" ;
    skos:prefLabel "Global Ecological Zones" .

fao:globalEcologicalZones2010 a skos:Concept ;
    skos:definition """
The GEZ spatial dataset used by FAO has developed over the years from covering only the tropical areas (1990) to the globe (2000). Due to the developments in remote sensing and the compiling of many spatial products relating to climate and land cover between 2000 and 2010, an update to the GEZ 2000 map was commissioned. This took the form of two months’ consultant work spread over ay-August 2011, and contributions from other scientists, particularly for North America and Australia. [https://www.fao.org/3/ap861e/ap861e.pdf]
""" ;
    skos:narrower fao:globalEcologicalZones ;
    skos:prefLabel "Global Ecological Zones 2010" .

fao:globalEcologicalZones2010Boreal a dct:Location,
        gsp:Feature,
        skos:Concept ;
    gsp:hasDefaultGeometry gez2010_geoms:boreal ;
    skos:definition "Up to 3 months over 10°C" ;
    skos:narrower fao:globalEcologicalZones2010 ;
    skos:prefLabel "Boreal Ecological Zones 2010" .

fao:globalEcologicalZones2010Polar a skos:Concept ;
    skos:definition "All months below 10°C" ;
    skos:narrower fao:globalEcologicalZones2010 ;
    skos:prefLabel "Polar Ecological Zones 2010" .

fao:globalEcologicalZones2010Subtropical a dct:Location,
        gsp:Feature,
        skos:Concept ;
    gsp:hasDefaultGeometry gez2010_geoms:subtropical ;
    skos:definition "Eight months or more over 10°C" ;
    skos:narrower fao:globalEcologicalZones2010 ;
    skos:prefLabel "Subtropical Ecological Zones 2010" .

fao:globalEcologicalZones2010TPolar a dct:Location,
        gsp:Feature ;
    gsp:hasDefaultGeometry gez2010_geoms:polar .

fao:globalEcologicalZones2010Temperate a dct:Location,
        gsp:Feature,
        skos:Concept ;
    gsp:hasDefaultGeometry gez2010_geoms:temperate ;
    skos:definition "Four to eight months over 10°C" ;
    skos:narrower fao:globalEcologicalZones2010 ;
    skos:prefLabel "Temperate Ecological Zones 2010" .

fao:globalEcologicalZones2010Tropical a dct:Location,
        gsp:Feature,
        skos:Concept ;
    gsp:hasDefaultGeometry gez2010_geoms:tropical ;
    skos:definition "All months without frost: in marine areas over 18°C" ;
    skos:narrower fao:globalEcologicalZones2010 ;
    skos:prefLabel "Tropical Ecological Zones 2010" .

fao:globalEcologicalZones2010Water a dct:Location,
        gsp:Feature,
        skos:Concept ;
    gsp:hasDefaultGeometry gez2010_geoms:water ;
    skos:narrower fao:globalEcologicalZones2010 ;
    skos:prefLabel "Global Ecological Zones 2010 - Water" .

